# TP 1 Calcul des Proposition

## Generalités

### Sous formules

- (a ∨ b) -> a ∨ b
- (a ∧ b) -> a ∧ b
- (e => f) -> e => f
- (e <=> f) -> e <=> f
- ¬i -> ¬i
- ((a => b) => b) => ¬(a ∨ b) -> a => b, a ∨ b, (a => b) => b, ¬(a ∨ b), ((a => b) => b) => (¬(a ∨ b))

### Table de vérité

| A | ¬A |
| - | -- |
| 0 | 1  |
| 1 | 0  |

| A | B | ∨ | ∧ | => | <=> |
| - | - | - | - | -- | --- |
| 0 | 0 | 0 | 0 | 1  | 1   |
| 0 | 1 | 1 | 0 | 1  | 0   |
| 1 | 0 | 1 | 0 | 0  | 0   |
| 1 | 1 | 1 | 1 | 1  | 1   | 

### Equivalence à ET et OU

| A | ¬A | B | ¬B | ∨ | ∧ | => | <=> |
| - | -- | - | -- | - | - | -- | --- |
| 0 | 1  | 0 | 1  | 0 | 0 | 1  | 1   |
| 0 | 1  | 1 | 0  | 1 | 0 | 1  | 0   |
| 1 | 0  | 0 | 1  | 1 | 0 | 0  | 0   |
| 1 | 0  | 1 | 0  | 1 | 1 | 1  | 1   | 


| A | B | ∧ | ¬(a=>¬b) |
| - | - | - | -------- |
| 0 | 0 | 0 | 0        |
| 0 | 1 | 0 | 0        | 
| 1 | 0 | 0 | 0		   |
| 1 | 1 | 1 | 1		   |



| A | B | ∨ | ¬a=>b |
| - | - | - | ----- |
| 0 | 0 | 0 | 0     |
| 0 | 1 | 0 | 0     | 
| 1 | 0 | 0 | 0	    |
| 1 | 1 | 1 | 1	    |

### Mise sous forme normale conhectives

(( a => (b ∨ c)) ∧ ((b ∨ d) => (e ∧ f))) ∧ ¬e

-> (( ¬a ∨ (a ∧ (b ∨ c))) ∧ (¬(b ∨ d)∨((b ∨ d)∧(e ∧ f)))) ∧ ¬e
-> (( ¬a ∨ ((a ∧ b) ∨ (a ∧ c)) ) ∧ (¬(b ∨ d) ∨ ( ((b ∨ d)∧e) ∨( (b ∨ d) ∧ f ))) ∧ ¬e
-> ( ( ))